src/spec/TLS13.ConnectionState.ProtectedWireServerFlight.fsti
@@ -129,6 +129,234 @@ val lemma_protected_handshake_event_projection_pair_after_server_write_client_re
             client_tail_received
             client_final)
 
+val lemma_protected_handshake_event_projection_pair_after_server_write_client_read_install_receiver_preserve_read_local_head_with_tails
+  (server:CS.connection_model)
+  (client:CS.connection_model)
+  (receiver_skip:CS.local_event)
+  (server_material:CS.traffic_key_material)
+  (client_material:CS.traffic_key_material)
+  (sent_msg:M.handshake_msg)
+  (received_msg:M.handshake_msg)
+  (server_rest:list CS.conn_event)
+  (client_rest:list CS.conn_event)
+  (server_raw_sent:B.bytes)
+  (server_raw_received:B.bytes)
+  (client_raw_sent:B.bytes)
+  (client_raw_received:B.bytes)
+  (server_final:CS.connection_model)
+  (client_final:CS.connection_model)
+  : Lemma
+      (requires
+        CS.record_key_iv_material_agrees
+          (CS.record_material_of_traffic_material server_material)
+          (CS.record_material_of_traffic_material client_material) /\
+        local_event_preserves_record_read receiver_skip /\
+        Seq.equal server_raw_sent client_raw_received /\
+        protected_handshake_wire_round_trip_message sent_msg /\
+        protected_handshake_wire_round_trip_message received_msg /\
+        CS.conn_events_sent_seal_replay
+          server
+          (CS.ConnLocalEvent
+            (CS.LocalInstallTrafficKeysForRole {
+              CS.install_role = CS.ServerEndpoint;
+              CS.install_payload = {
+                CS.install_epoch = CS.TrafficHandshake;
+                CS.install_direction = CS.TrafficWrite;
+                CS.install_material = server_material;
+              };
+            }) :: CS.ConnNetworkEvent {
+              CL.message_direction = CL.Sent;
+              CL.message_value = M.TlsHandshake sent_msg;
+            } :: server_rest)
+          server_raw_sent
+          server_raw_received
+          server_final /\
+        CS.conn_events_received_decode_replay
+          client
+          (CS.ConnLocalEvent
+            (CS.LocalInstallTrafficKeys {
+              CS.install_epoch = CS.TrafficHandshake;
+              CS.install_direction = CS.TrafficRead;
+              CS.install_material = client_material;
+            }) :: CS.ConnLocalEvent receiver_skip :: CS.ConnNetworkEvent {
+              CL.message_direction = CL.Received;
+              CL.message_value = M.TlsHandshake received_msg;
+            } :: client_rest)
+          client_raw_sent
+          client_raw_received
+          client_final)
+      (ensures
+        exists server_after client_after client_after_skip
+          server_after_head client_after_head pair
+          server_tail_sent server_tail_received
+          client_tail_sent client_tail_received.
+          CS.step_model
+            server
+            (CS.ConnLocalEvent
+              (CS.LocalInstallTrafficKeysForRole {
+                CS.install_role = CS.ServerEndpoint;
+                CS.install_payload = {
+                  CS.install_epoch = CS.TrafficHandshake;
+                  CS.install_direction = CS.TrafficWrite;
+                  CS.install_material = server_material;
+                };
+              })) == Some server_after /\
+          CS.step_model
+            client
+            (CS.ConnLocalEvent
+              (CS.LocalInstallTrafficKeys {
+                CS.install_epoch = CS.TrafficHandshake;
+                CS.install_direction = CS.TrafficRead;
+                CS.install_material = client_material;
+              })) == Some client_after /\
+          CS.step_model client_after (CS.ConnLocalEvent receiver_skip) ==
+            Some client_after_skip /\
+          CS.step_model
+            server_after
+            (CS.ConnNetworkEvent {
+              CL.message_direction = CL.Sent;
+              CL.message_value = M.TlsHandshake sent_msg;
+            }) == Some server_after_head /\
+          CS.step_model
+            client_after_skip
+            (CS.ConnNetworkEvent {
+              CL.message_direction = CL.Received;
+              CL.message_value = M.TlsHandshake received_msg;
+            }) == Some client_after_head /\
+          pair.pm_sender == server_after /\
+          pair.pm_receiver == client_after_skip /\
+          protected_handshake_event_projection_pair
+            pair
+            sent_msg
+            received_msg /\
+          Seq.equal server_tail_sent client_tail_received /\
+          CS.conn_events_sent_seal_replay
+            server_after_head
+            server_rest
+            server_tail_sent
+            server_tail_received
+            server_final /\
+          CS.conn_events_received_decode_replay
+            client_after_head
+            client_rest
+            client_tail_sent
+            client_tail_received
+            client_final)
+
+val lemma_protected_handshake_event_projection_pair_after_server_write_receiver_preserve_read_local_head_client_read_install_with_tails
+  (server:CS.connection_model)
+  (client:CS.connection_model)
+  (receiver_skip:CS.local_event)
+  (server_material:CS.traffic_key_material)
+  (client_material:CS.traffic_key_material)
+  (sent_msg:M.handshake_msg)
+  (received_msg:M.handshake_msg)
+  (server_rest:list CS.conn_event)
+  (client_rest:list CS.conn_event)
+  (server_raw_sent:B.bytes)
+  (server_raw_received:B.bytes)
+  (client_raw_sent:B.bytes)
+  (client_raw_received:B.bytes)
+  (server_final:CS.connection_model)
+  (client_final:CS.connection_model)
+  : Lemma
+      (requires
+        CS.record_key_iv_material_agrees
+          (CS.record_material_of_traffic_material server_material)
+          (CS.record_material_of_traffic_material client_material) /\
+        local_event_preserves_record_read receiver_skip /\
+        Seq.equal server_raw_sent client_raw_received /\
+        protected_handshake_wire_round_trip_message sent_msg /\
+        protected_handshake_wire_round_trip_message received_msg /\
+        CS.conn_events_sent_seal_replay
+          server
+          (CS.ConnLocalEvent
+            (CS.LocalInstallTrafficKeysForRole {
+              CS.install_role = CS.ServerEndpoint;
+              CS.install_payload = {
+                CS.install_epoch = CS.TrafficHandshake;
+                CS.install_direction = CS.TrafficWrite;
+                CS.install_material = server_material;
+              };
+            }) :: CS.ConnNetworkEvent {
+              CL.message_direction = CL.Sent;
+              CL.message_value = M.TlsHandshake sent_msg;
+            } :: server_rest)
+          server_raw_sent
+          server_raw_received
+          server_final /\
+        CS.conn_events_received_decode_replay
+          client
+          (CS.ConnLocalEvent receiver_skip :: CS.ConnLocalEvent
+            (CS.LocalInstallTrafficKeys {
+              CS.install_epoch = CS.TrafficHandshake;
+              CS.install_direction = CS.TrafficRead;
+              CS.install_material = client_material;
+            }) :: CS.ConnNetworkEvent {
+              CL.message_direction = CL.Received;
+              CL.message_value = M.TlsHandshake received_msg;
+            } :: client_rest)
+          client_raw_sent
+          client_raw_received
+          client_final)
+      (ensures
+        exists server_after client_after_skip client_after
+          server_after_head client_after_head pair
+          server_tail_sent server_tail_received
+          client_tail_sent client_tail_received.
+          CS.step_model
+            server
+            (CS.ConnLocalEvent
+              (CS.LocalInstallTrafficKeysForRole {
+                CS.install_role = CS.ServerEndpoint;
+                CS.install_payload = {
+                  CS.install_epoch = CS.TrafficHandshake;
+                  CS.install_direction = CS.TrafficWrite;
+                  CS.install_material = server_material;
+                };
+              })) == Some server_after /\
+          CS.step_model client (CS.ConnLocalEvent receiver_skip) ==
+            Some client_after_skip /\
+          CS.step_model
+            client_after_skip
+            (CS.ConnLocalEvent
+              (CS.LocalInstallTrafficKeys {
+                CS.install_epoch = CS.TrafficHandshake;
+                CS.install_direction = CS.TrafficRead;
+                CS.install_material = client_material;
+              })) == Some client_after /\
+          CS.step_model
+            server_after
+            (CS.ConnNetworkEvent {
+              CL.message_direction = CL.Sent;
+              CL.message_value = M.TlsHandshake sent_msg;
+            }) == Some server_after_head /\
+          CS.step_model
+            client_after
+            (CS.ConnNetworkEvent {
+              CL.message_direction = CL.Received;
+              CL.message_value = M.TlsHandshake received_msg;
+            }) == Some client_after_head /\
+          pair.pm_sender == server_after /\
+          pair.pm_receiver == client_after /\
+          protected_handshake_event_projection_pair
+            pair
+            sent_msg
+            received_msg /\
+          Seq.equal server_tail_sent client_tail_received /\
+          CS.conn_events_sent_seal_replay
+            server_after_head
+            server_rest
+            server_tail_sent
+            server_tail_received
+            server_final /\
+          CS.conn_events_received_decode_replay
+            client_after_head
+            client_rest
+            client_tail_sent
+            client_tail_received
+            client_final)
+
 val lemma_protected_handshake_event_projection_pair_after_server_write_client_read_install_heads_with_next_alignment_and_tails
   (server:CS.connection_model)
   (client:CS.connection_model)
